ADD: new operations; EDIT: execution grammar

Exec.fst
@@ -1,74 +1,118 @@
 module Exec
 
 (*
-   Req: true
-*)
-let check_err dataStack = 
-  match (List.length dataStack) with
-  | 0 -> None
-  | _ ->
-    match (List.hd dataStack) with
-    | ERR(s) -> Some (ERR(s))
-    | _ -> None
-    
-(*
-   Req: length(datastack) >= 1
-*)
-let return_value dataStack = List.hd dataStack
+Notaion: 
+  - tos means top of stack (i.e., datastack[0])
+    - for the second elemnt in the stack and the elements following it:
+      - The (i+1)th element is represtned as tosi
+      - eg: 2nd element = tos1, 3rd element = tos2, ...
+  
+  - BOOL(b): b in F* is true or false, but in python evaluation it'streated as int
+    - True = 1 and False = 0
+    - So in req and Ens b in BOOL(b) is just 1 or 0
+
+  - res is what a function evaluates to. 
+*) 
+
+(* Create a new frame and push it in the frame stack *)
+let makeFrame virM code localplus global_names local_names =
+  let frame: frameObj = {
+    dataStack = []; 
+    blockStack = [];
+    fCode = code;
+    f_localplus = localplus;
+    pc = 0;
+    f_globals = global_names;
+    f_locals = local_names
+  } in
+  let newVM: vm = {virM with callStack = frame::(virM.callStack)} in
+  (newVM, frame)
 
 (*
+  Req:
+  Ens:
+*)
+let call_function i globals dataStack =
+  let args, newDataStack = List.splitAt i dataStack in
+  let localplus = List.Tot.Base.rev args in
+  let code, newDataStack = List.splitAt 1 newDataStack in
+  let empty_map = Map.const_on (Set.empty) NONE in
+  match List.hd code with
+  | CODEOBJECT co ->  
+    let newFrame: frameObj = {
+      dataStack = []; 
+      blockStack = [];
+      fCode = co;
+      f_localplus = localplus;
+      pc = 0;
+      f_globals = globals;
+      f_locals = empty_map
+    } in (FRAMEOBJECT newFrame)::dataStack
+  | _ -> All.failwith "CALL_FUNCTION: didn't call a function object"
+  
+(*
    Req: length(datastack) >= 1
+   Ens: res = datastack[1:]
 *)
 let pop_top datastack = List.tail datastack
 
 (*
    Req: length(datastack) >= 2
+   Ens: res = tos1::tos::datastack[2:]
 *)
 let rot_two datastack = 
-  let fst_elem = List.hd datastack in
-  let scnd_elem = List.nth datastack 1 in
+  let tos = List.hd datastack in
+  let tos1 = List.nth datastack 1 in
   let _, rest_stack = List.splitAt 2 datastack in
-  scnd_elem::fst_elem::rest_stack
+  tos1::tos::rest_stack
 
 (*
    Req: length(datastack) >= 3
+   Ens: res = tos1::tos2::tos::datastack[3:]
 *)
 let rot_three datastack = 
-  let fst_elem = List.hd datastack in
-  let scnd_elem = List.nth datastack 1 in
-  let thrd_elem = List.nth datastack 2 in
+  let tos = List.hd datastack in
+  let tos1 = List.nth datastack 1 in
+  let tos2 = List.nth datastack 2 in
   let _, rest_stack = List.splitAt 3 datastack in
-  scnd_elem::thrd_elem::fst_elem::rest_stack
+  tos1::tos2::tos::rest_stack
 
 (*
    Req: length(datastack) >= 4
+   Ens: res = tos1::tos2::tos3::tos::datastack[4:]
 *)
 let rot_four datastack = 
-  let fst_elem = List.hd datastack in
-  let scnd_elem = List.nth datastack 1 in
-  let thrd_elem = List.nth datastack 2 in
-  let frth_elem = List.nth datastack 3 in
+  let tos = List.hd datastack in
+  let tos1 = List.nth datastack 1 in
+  let tos2 = List.nth datastack 2 in
+  let tos3 = List.nth datastack 3 in
   let _, rest_stack = List.splitAt 4 datastack in
-  scnd_elem::thrd_elem::frth_elem::fst_elem::rest_stack
+  tos1::tos2::tos3::tos::rest_stack
 
 (*
    Req: length(datastack) >= 1
+   Ens: res = tos::datastack
 *)
 let dup_top datastack = 
-  let fst_elem = List.hd datastack in
-  fst_elem::datastack
+  let tos = List.hd datastack in
+  tos::datastack
 
 (*
    Req: length(datastack) >= 2
+   Ens: res = tos::tos1::datastack
 *)
 let dup_top_two datastack = 
-  let fst_elem = List.hd datastack in
-  let scnd_elem = List.nth datastack 1 in
-  fst_elem::scnd_elem::datastack
+  let tos = List.hd datastack in
+  let tos1 = List.nth datastack 1 in
+  tos::tos1::datastack
 
 
 (*
    Req: length(datastack) >= 1
+   Ens: 
+     - if tos = INT(i) then res = INT(+i)
+     - if tos = BOOL(b) then res = INT(if b then 1 else 0)
+     - else ERR
 *)
 let unary_positive datastack = 
   let tos = List.hd datastack in
@@ -80,6 +124,10 @@ let unary_positive datastack =
 
 (*
    Req: length(datastack) >= 1
+   Ens: 
+     - if tos = INT(i) then res = INT(-i)
+     - if tos = BOOL(b) then res = INT(if b then -1 else 0)
+     - else ERR
 *)
 let unary_negative datastack = 
   let tos = List.hd datastack in
@@ -91,6 +139,11 @@ let unary_negative datastack =
 
 (*
    Req: length(datastack) >= 1
+   Ens:
+     - if tos = INT(i)
+     - if tos = STRING(s)
+     - if tos = BOOL(b)
+     - if tos = NONE 
 *)
 let unary_not datastack = 
   let tos = List.hd datastack in
@@ -99,11 +152,20 @@ let unary_not datastack =
   | INT i -> BOOL(if i=0 then true else false)::newDataStack
   | STRING s -> BOOL(if s="" then true else false)::newDataStack
   | BOOL b -> BOOL(if b then false else true)::newDataStack
+  | LIST l -> BOOL(match l with [] -> true | _ -> false)::newDataStack
+  | TUPLE t -> BOOL(match t with [] -> true | _ -> false)::newDataStack
   | NONE -> BOOL(true)::newDataStack
   | _ -> ERR("Error: bad operand type for unary -")::newDataStack
 
 (*
   Req: length(datastack) >= 2
+  Ens:
+    - if tos and tos1 are int(i1), int(i2) or bool(b1), bool(b2):
+      - res = i1*i2, or res = b1 * b2
+    - if tos and tos1 are List(l), int(i) or List(l), bool(b):
+      - res = a list of the items of l repeated i (or b) times
+      - if i <= 0 then res = []
+    - else: res = ERR
 *)
 let binary_multiply (dataStack: list pyObj) = 
   let tos = List.hd dataStack in
@@ -112,13 +174,37 @@ let binary_multiply (dataStack: list pyObj) =
   match (tos, tos1) with
   | INT(i1), INT(i2) -> INT(op_Multiply i2 i1)::newDataStack
   | BOOL(b1), BOOL(b2) -> INT(if b1&&b2 then 1 else 0)::newDataStack
-  | BOOL(b1), INT(i) -> INT(if b1 then i else  0)::newDataStack
-  | INT(i), BOOL(b2) -> INT(if b2 then i else 0)::newDataStack
+  | BOOL(b), INT(i) -> INT(if b then i else  0)::newDataStack
+  | INT(i), BOOL(b) -> INT(if b then i else 0)::newDataStack
+  | LIST(l), INT(i) ->
+    if 0 >= i 
+    then LIST([])::newDataStack
+    else
+      let l' = List.fold_left (fun x y -> List.append x y) ([]) (tabulate (fun x -> l) i) in
+      LIST(l')::newDataStack
+  | INT(i), LIST(l) -> 
+    if 0 >= i 
+    then LIST([])::newDataStack
+    else
+      let l' = List.fold_left (fun x y -> List.append x y) ([]) (tabulate (fun x -> l) i) in
+      LIST(l')::newDataStack
+  | LIST(l), BOOL(b) -> if b then LIST(l)::newDataStack else LIST([])::newDataStack
+  | BOOL(b), LIST(l) -> if b then LIST(l)::newDataStack else LIST([])::newDataStack
+  | TUPLE(t), INT(i) ->
+    if 0 >= i 
+    then TUPLE([])::newDataStack
+    else
+      let t' = List.fold_left (fun x y -> List.append x y) ([]) (tabulate (fun x -> t) i) in
+      TUPLE(t')::newDataStack
+  | TUPLE(t), BOOL(b) -> if b then TUPLE(t)::newDataStack else TUPLE([])::newDataStack  
   | _, _ -> ERR("Error: unsupported operand type(s) for *")::newDataStack
 
 (*
   Req: length(datastack) >= 2
-  ENS: (tos = tos1 // tos) or (tos = ERR)
+  ENS:
+    - if tos and tos1 are int(a), int(b) or bool(b1), bool(b2)
+      - res = b // a (or b2 // b1) if a <> 0 (or b1 <> 0)
+      - res = ERR if a == 0 (or b1 == 0)
 *)
 let binary_floor_divide (dataStack: list pyObj) = 
   let tos = List.hd dataStack in
@@ -133,7 +219,10 @@ let binary_floor_divide (dataStack: list pyObj) =
 
 (*
   Req: length(datastack) >= 2
-  ENS: (tos = tos1 % tos) or (tos = ERR)
+  ENS:
+    - if tos and tos1 are int(a), int(b) or bool(b1), bool(b2)
+      - res = b % a (or b2 % b1) if a <> 0 (or b1 <> 0)
+      - res = ERR if a == 0 (or b1 == 0)
 *)
 let binary_modulo (dataStack: list pyObj) = 
   let tos = List.hd dataStack in
@@ -145,9 +234,20 @@ let binary_modulo (dataStack: list pyObj) =
   | INT(i), BOOL(b2) -> (if i=0 then ERR("Error: modulo by zero") else if b2 then INT(1%i) else INT(0%i))::newDataStack
   | BOOL(b1), INT(i) -> (if not b1 then ERR("Error: modulo by zero") else INT(i%1))::newDataStack
   | _, _ -> ERR("Error: unsupported operand type(s) for %")::newDataStack
-  
+
 (*
   Req: length(datastack) >= 2
+  Ens: 
+    - if tos and tos1 are INT(i1)/BOOL(b1) and INT(i2)/BOOL(b2):
+      - res = INT(i1 + i2) (or b1,b2)
+    - if tos and tos1 are STRING(s1) and STRING(s2):
+      - res = STRING(s1 ^ s2)
+    - if tos and tos1 are LIST(l1) and LIST(l2):
+      - res = LIST(l1 @ l2)
+    - if tos and tos1 are TUPLE(t1) and TUPLE(t2):
+      - res = TUPLE(t1 @ t2)
+    - else:
+      - res = ERR
 *)
 let binary_add (dataStack: list pyObj) = 
   let tos = List.hd dataStack in
@@ -159,10 +259,17 @@ let binary_add (dataStack: list pyObj) =
   | BOOL(b1), INT(i) -> INT(if b1 then 1+i else  0+i)::newDataStack
   | INT(i), BOOL(b2) -> INT(if b2 then 1+i else 0+i)::newDataStack
   | STRING(s1), STRING(s2) -> STRING(s2 ^  s1)::newDataStack
+  | LIST(l1), LIST(l2) -> LIST(List.append l1 l2)::newDataStack
+  | TUPLE(t1), TUPLE(t2) -> LIST(List.append t1 t2)::newDataStack
   | _, _ -> ERR("Error: unsupported operand type(s) for +")::newDataStack
-  
+ 
 (*
   Req: length(datastack) >= 2
+  Ens:
+    - if tos and tos1 are INT(i1) and INT(i2) or(BOOL(b1) and BOOL(b2)):
+      - res = INT(i2 - i1), or(b1, b2)
+    - else:
+      - res = ERR
 *)
 let binary_subtract (dataStack: list pyObj) = 
   let tos = List.hd dataStack in
@@ -176,7 +283,71 @@ let binary_subtract (dataStack: list pyObj) =
   | _, _ -> ERR("Error: unsupported operand type(s) for -")::newDataStack
   
 (*
+  Req: length(datastack) >= 2
+  Ens: TOS = TOS1[TOS]
+*)
+let binary_subscr (dataStack: list pyObj) = 
+  let tos = List.hd dataStack in
+  let tos1 = List.nth dataStack 1 in
+  let (_, newDataStack) = List.splitAt 2 dataStack in 
+  match (tos1, tos) with
+  | STRING(s), INT(i) ->
+    let c = if i >= 0 then (subString_pos s i) else (subString_neg s i) in
+     ( match c with
+      | Some c' -> STRING(c')::newDataStack
+      | None -> ERR("Error: String index out of range")::newDataStack)
+  | STRING(s), BOOL(b) -> 
+    let c = if b then (subString_pos s 1) else (subString_neg s 0) in
+      (match c with
+      | Some c' -> STRING(c')::newDataStack
+      | None -> ERR("Error: String index out of range")::newDataStack)
+  | LIST(l), INT(i) -> 
+    let e = 
+      if i >= 0 then (List.Tot.Base.nth l i)
+      else if (-i > List.length l) then None
+      else (List.Tot.Base.nth l ((List.length l) - i))
+    in
+     ( match e with
+      | Some e' -> e'::newDataStack
+      | None ->  ERR("Error: List index out of range")::newDataStack)
+  | LIST(l), BOOL(b) ->
+    let e = if b then (List.Tot.Base.nth l 1) else (List.Tot.Base.nth l 0) in
+     ( match e with
+      | Some e' -> e'::newDataStack
+      | None -> ERR("Error: List index out of range")::newDataStack)
+  | TUPLE(t), INT(i) ->
+    let e = 
+      if i >= 0 then (List.Tot.Base.nth t i)
+      else if (-i > List.length t) then None
+      else (List.Tot.Base.nth t ((List.length t) - i))
+    in
+     ( match e with
+      | Some e' -> e'::newDataStack
+      | None ->  ERR("Error: Tuple index out of range")::newDataStack)
+  | TUPLE(t), BOOL(b) ->
+    let e = if b then (List.Tot.Base.nth t 1) else (List.Tot.Base.nth t 0) in
+      (match e with
+      | Some e' -> e'::newDataStack
+      | None -> ERR("Error: Tuple index out of range")::newDataStack)
+  | _, _ -> ERR("Error: object is not subscriptable")::newDataStack
+  
+(*
+  Req:
+  Ens:
+*)
+let store_name i names f_locals dataStack = 
+  let name = List.nth names i in
+  let tos = List.hd dataStack in
+  let _, newDataStack = List.splitAt 1 dataStack in 
+  (match name with
+  | STRING s -> 
+    let newLocals = Map.upd f_locals s tos in
+    (newLocals, newDataStack)
+  | _ -> All.failwith "STORE_NAME: co_names[i] is not STRING")
+  
+(*
   Req: (length(consts) > i) && (length(datastack) >= 1)
+  Ens: res = consts[i]::datastack
 *)
 let load_const i consts dataStack =
   let elem = List.nth consts i in
@@ -184,151 +355,296 @@ let load_const i consts dataStack =
   newDataStack
 
 (*
-  Req: (length(varnames) > i) && (length(datastack) >= 1)
+  Req:
+  Ens:
 *)
-let load_fast i varnames dataStack =
-  let elem = List.nth varnames i in
+let load_name i names f_locals f_globals dataStack =
+  let name = List.nth names i in
+  match name with
+  | STRING s ->
+    (match Map.contains f_locals s with
+     | true -> (Map.sel f_locals s)::dataStack 
+     | false ->
+       (match Map.contains f_globals s with
+        | true -> (Map.sel f_locals s)::dataStack
+        | false -> (ERR ("name " ^ s ^ "is not defined"))::dataStack
+       )
+    )
+  | _ -> All.failwith "LOAD_NAME: co_names[i] is not STRING"
+ 
+(*
+  Req: (length(datastack) >= i)
+  Ens: res = LIST([dataStack[0]; dataStack[1], ... dataStrack[i-1]])::newDataStack
+*)
+let build_tuple i dataStack =
+  let elems, newDataStack  = List.splitAt i dataStack in
+  let newDataStack = TUPLE(elems)::newDataStack in
+  newDataStack
+
+(*
+  Req: (length(datastack) >= i)
+  Ens: res = TUPLE([dataStack[0]; dataStack[1], ... dataStrack[i-1]])::newDataStack
+*)
+let build_list i dataStack =
+  let elems, newDataStack  = List.splitAt i dataStack in
+  let newDataStack = LIST(elems)::newDataStack in
+  newDataStack
+
+(*
+  Req:
+  Ens:
+*)
+let pop_jump_if_true i pc dataStack =
+  let tos = List.hd dataStack in
+  let newDataStack = List.tail dataStack in
+  match tos with
+  | BOOL b -> if b then (i/2, newDataStack) else (pc, newDataStack)
+  | _ -> (pc, (ERR "ERR: argument is not a Bool")::newDataStack)
+
+(*
+  Req:
+  Ens:
+*)
+let pop_jump_if_false i pc dataStack =
+  let tos = List.hd dataStack in
+  let newDataStack = List.tail dataStack in
+  match tos with
+  | BOOL b -> if b then (pc, newDataStack) else (i/2, newDataStack)
+  | _ -> (pc, (ERR "ERR: argument is not a Bool")::newDataStack)
+
+(*
+  Req:
+  Ens:
+*)
+let jump_if_true_or_pop i pc dataStack =
+  let tos = List.hd dataStack in
+  let newDataStack = List.tail dataStack in
+  match tos with
+  | BOOL b -> if b then (i/2, dataStack) else (pc, newDataStack)
+  | _ -> (pc, (ERR "ERR: argument is not a Bool")::newDataStack)
+
+(*
+  Req:
+  Ens:
+*)
+let jump_if_false_or_pop i pc dataStack =
+  let tos = List.hd dataStack in
+  let newDataStack = List.tail dataStack in
+  match tos with
+  | BOOL b -> if b then (pc, newDataStack) else (i/2, dataStack)
+  | _ -> (pc, (ERR "ERR: argument is not a Bool")::newDataStack)
+ 
+(*
+  Req:
+  Ens:
+*)
+let load_global i names f_globals dataStack =
+  let name = List.nth names i in
+  match name with
+  | STRING s ->
+    (match Map.contains f_globals s with
+     | true -> (Map.sel f_globals s)::dataStack 
+     | false -> (ERR ("name " ^ s ^ "is not defined"))::dataStack
+    )
+  | _ -> All.failwith "LOAD_GLOBAL: co_names[i] is not STRING"
+
+(*
+  Req: (length(localplus) > i) && (length(datastack) >= 1)
+  Ens: res = localplus[i]::dataStack
+*)
+let load_fast i localPlus dataStack =
+  let elem = List.nth localPlus i in
   let newDataStack = elem::dataStack in
   newDataStack
 
 (*
-  Req: (length(varnames) > i) && (length(datastack) >= 1)
+  Req: i >= (length(f_localplus)) && (length(datastack) >= 1)
+  Ens: res = (localplus where localplus[i] = tos, datastack[1:])
 *)
-let store_fast i varnames dataStack =
-  let elem = List.hd dataStack in
+let store_fast i localplus dataStack =
+  let tos = List.hd dataStack in
   let newDataStack = List.tail dataStack in
-  let newVarnames = List.mapi (fun k x -> if k = i then elem else x) varnames in
-  (newVarnames, newDataStack)
-
+    match (List.Tot.Base.length localplus) > i with
+    | true ->
+      (let newLocalPlus = List.mapi (fun k x -> if k = i then tos else x) localplus in
+        (newLocalPlus, newDataStack))
+    | false ->
+      (match (List.Tot.Base.length localplus) = i with
+       | true ->
+         (let newLocalPlus = List.append localplus [tos] in
+           (newLocalPlus, newDataStack)) 
+       | false -> All.failwith "STORE_FAST: storing out of index")
+  
+(*
+  Req:
+  Ens:
+*)
+let make_function flags globs dataStack =
+  let qualname = List.hd dataStack in
+  let codeobj = List.nth dataStack 1 in
+  let (_, newDataStack) = List.splitAt 2 dataStack in 
+  let func = FUNCTION ({
+    func_Code = codeobj;
+    func_globals = globs;
+    func_name = qualname;
+    func_closure =
+      if flags = 8 then
+      (match List.hd newDataStack with
+       | TUPLE(t) -> TUPLE(t)
+       | _ -> ERR "Expected closure tuple, got someting else") else NONE;
+   
+    func_defaults =
+      if flags = 1 then
+      (match  List.hd newDataStack with
+       | TUPLE(t) -> TUPLE(t)
+       | _ -> ERR "Expected a defaults tuple, got someting else") else NONE;
+  }) in
+    (match flags with
+     | 0 -> func::newDataStack
+     | _ -> func::(List.tail newDataStack))
+     
 (*
    Req: len(frame.fcode.bytecode) >= 1
 *)
 let rec execBytecode frame =
-  let CODE(bc) = frame.fCode.co_code in
-  match bc with
-  | RETURN_VALUE::l -> return_value frame.dataStack
-
-  | NOP::l -> execBytecode ({frame with fCode = {frame.fCode with co_code = CODE l}})
-
-  | POP_TOP::l ->
-    let newDataStack = pop_top frame.dataStack in
-    let errCheck = check_err newDataStack in (
-    match errCheck with
-    | Some err -> err
-    | None -> execBytecode ({frame with dataStack = newDataStack; fCode = {frame.fCode with co_code = CODE l}}))
+  match check_err frame.dataStack with
+  | Some err -> frame
+  | None -> 
   
-  | ROT_TWO::l ->
-    let newDataStack = rot_two frame.dataStack in
-    let errCheck = check_err newDataStack in (
-    match errCheck with
-    | Some err -> err
-    | None -> execBytecode ({frame with dataStack = newDataStack; fCode = {frame.fCode with co_code = CODE l}}))
-   
-  | ROT_THREE::l ->
-    let newDataStack = rot_three frame.dataStack in
-    let errCheck = check_err newDataStack in (
-    match errCheck with
-    | Some err -> err
-    | None -> execBytecode ({frame with dataStack = newDataStack; fCode = {frame.fCode with co_code = CODE l}}))
-   
-  | ROT_FOUR::l ->
-    let newDataStack = rot_four frame.dataStack in
-    let errCheck = check_err newDataStack in (
-    match errCheck with
-    | Some err -> err
-    | None -> execBytecode ({frame with dataStack = newDataStack; fCode = {frame.fCode with co_code = CODE l}}))
+    let CODE(bc) = frame.fCode.co_code in
+    match List.nth bc (frame.pc) with
+    | RETURN_VALUE -> frame
+    | CALL_FUNCTION i -> 
+      let newDataStack = call_function i (frame.f_globals) frame.dataStack in
+        ({frame with dataStack = newDataStack})
+    | NOP -> execBytecode ({frame with pc = frame.pc+1})
+    | POP_TOP ->
+      let newDataStack = pop_top frame.dataStack in
+        execBytecode ({frame with dataStack = newDataStack; pc = frame.pc+1})
+    | ROT_TWO ->
+      let newDataStack = rot_two frame.dataStack in
+        execBytecode ({frame with dataStack = newDataStack; pc = frame.pc+1})
+    | ROT_THREE ->
+      let newDataStack = rot_three frame.dataStack in
+        execBytecode ({frame with dataStack = newDataStack; pc = frame.pc+1})
+    | ROT_FOUR ->
+      let newDataStack = rot_four frame.dataStack in
+        execBytecode ({frame with dataStack = newDataStack; pc = frame.pc+1})
+    | DUP_TOP ->
+      let newDataStack = dup_top frame.dataStack in
+        execBytecode ({frame with dataStack = newDataStack; pc = frame.pc+1})
+    | DUP_TOP_TWO ->
+      let newDataStack = dup_top_two frame.dataStack in
+        execBytecode ({frame with dataStack = newDataStack; pc = frame.pc+1})
+    | UNARY_POSITIVE ->
+      let newDataStack = unary_positive frame.dataStack in
+        execBytecode ({frame with dataStack = newDataStack; pc = frame.pc+1})
+    | UNARY_NEGATIVE ->
+      let newDataStack = unary_negative frame.dataStack in
+        execBytecode ({frame with dataStack = newDataStack; pc = frame.pc+1})
+    | UNARY_NOT ->
+      let newDataStack = unary_not frame.dataStack in
+        execBytecode ({frame with dataStack = newDataStack; pc = frame.pc+1})
+    | BINARY_MULTIPLY -> 
+      let newDataStack = binary_multiply (frame.dataStack) in
+        execBytecode ({frame with dataStack = newDataStack; pc = frame.pc+1})
+    | BINARY_FLOOR_DIVIDE -> 
+      let newDataStack = binary_floor_divide (frame.dataStack) in
+        execBytecode ({frame with dataStack = newDataStack; pc = frame.pc+1})    
+    | BINARY_MODULO -> 
+      let newDataStack = binary_modulo (frame.dataStack) in
+        execBytecode ({frame with dataStack = newDataStack; pc = frame.pc+1})
+    | BINARY_ADD -> 
+      let newDataStack = binary_add (frame.dataStack) in
+        execBytecode ({frame with dataStack = newDataStack; pc = frame.pc+1})    
+    | BINARY_SUBTRACT -> 
+      let newDataStack = binary_subtract (frame.dataStack) in
+        execBytecode ({frame with dataStack = newDataStack; pc = frame.pc+1}) 
+    | BINARY_SUBSCR -> 
+      let newDataStack = binary_subtract (frame.dataStack) in
+        execBytecode ({frame with dataStack = newDataStack; pc = frame.pc+1}) 
+    | LOAD_CONST(i) ->
+      let newDataStack = load_const i (frame.fCode.co_consts) (frame.dataStack) in
+        execBytecode ({frame with dataStack = newDataStack; pc = frame.pc+1})
+    | LOAD_NAME(i) ->
+      let newDataStack = load_name i (frame.fCode.co_names) (frame.f_locals) (frame.f_globals) (frame.dataStack) in
+        execBytecode ({frame with dataStack = newDataStack; pc = frame.pc+1})
+    | BUILD_TUPLE(i) ->
+      let newDataStack = build_tuple i (frame.dataStack) in
+        execBytecode ({frame with dataStack = newDataStack; pc = frame.pc+1})
+    | STORE_NAME(i) ->
+      let newLocals, newDataStack = store_name i (frame.fCode.co_names) (frame.f_locals) (frame.dataStack) in
+        execBytecode ({frame with dataStack = newDataStack; pc = frame.pc+1; f_locals = newLocals})
+    |  BUILD_LIST(i) ->
+      let newDataStack = build_list i (frame.dataStack) in
+        execBytecode ({frame with dataStack = newDataStack; pc = frame.pc+1})
+    | JUMP_FORWARD(i) -> execBytecode ({frame with pc = frame.pc + (i/2) + 1})
+    | POP_JUMP_IF_TRUE(i) ->
+      let newPc, newDataStack = pop_jump_if_true i (frame.pc) (frame.dataStack) in
+      let newPc = if frame.pc=newPc then newPc+1 else newPc in
+        execBytecode ({frame with dataStack = newDataStack; pc = newPc})
+    | POP_JUMP_IF_FALSE(i) ->
+      let newPc, newDataStack = pop_jump_if_false i (frame.pc) (frame.dataStack) in
+      let newPc = if frame.pc=newPc then newPc+1 else newPc in
+        execBytecode ({frame with dataStack = newDataStack; pc = newPc})
+    | JUMP_IF_TRUE_OR_POP(i) ->
+      let newPc, newDataStack = jump_if_true_or_pop i (frame.pc) (frame.dataStack) in
+      let newPc = if frame.pc=newPc then newPc+1 else newPc in
+        execBytecode ({frame with dataStack = newDataStack; pc = newPc})
+    | JUMP_IF_FALSE_OR_POP(i) ->
+      let newPc, newDataStack = jump_if_false_or_pop i (frame.pc) (frame.dataStack) in
+      let newPc = if frame.pc=newPc then newPc+1 else newPc in
+        execBytecode ({frame with dataStack = newDataStack; pc = newPc})
+    | JUMP_ABSOLUTE(i) -> execBytecode ({frame with pc = i/2})
+    | LOAD_GLOBAL(i) ->
+      let newDataStack = load_global i (frame.fCode.co_names) (frame.f_globals) (frame.dataStack) in
+        execBytecode ({frame with dataStack = newDataStack; pc = frame.pc+1})
+    | LOAD_FAST(i) ->
+      let newDataStack = load_fast i (frame.f_localplus) (frame.dataStack) in
+        execBytecode ({frame with dataStack = newDataStack; pc = frame.pc+1})   
+    | STORE_FAST(i) ->
+      let newLocalPlus, newDataStack = store_fast i (frame.f_localplus) (frame.dataStack) in
+        execBytecode ({frame with dataStack = newDataStack; pc = frame.pc+1; f_localplus = newLocalPlus})
+    | MAKE_FUNCTION(flags) ->
+      let newDataStack = make_function flags (frame.f_globals) (frame.dataStack) in
+        execBytecode ({frame with dataStack = newDataStack; pc = frame.pc+1})
+   | _ -> All.failwith "daa"
 
-  | DUP_TOP::l ->
-    let newDataStack = dup_top frame.dataStack in
-    let errCheck = check_err newDataStack in (
-    match errCheck with
-    | Some err -> err
-    | None -> execBytecode ({frame with dataStack = newDataStack; fCode = {frame.fCode with co_code = CODE l}}))
-
-  | DUP_TOP_TWO::l ->
-    let newDataStack = dup_top_two frame.dataStack in
-    let errCheck = check_err newDataStack in (
-    match errCheck with
-    | Some err -> err
-    | None -> execBytecode ({frame with dataStack = newDataStack; fCode = {frame.fCode with co_code = CODE l}}))
-
-  | UNARY_POSITIVE::l ->
-    let newDataStack = unary_positive frame.dataStack in
-    let errCheck = check_err newDataStack in (
-    match errCheck with
-    | Some err -> err
-    | None -> execBytecode ({frame with dataStack = newDataStack; fCode = {frame.fCode with co_code = CODE l}}))
-
-  | UNARY_NEGATIVE::l ->
-    let newDataStack = unary_negative frame.dataStack in
-    let errCheck = check_err newDataStack in (
-    match errCheck with
-    | Some err -> err
-    | None -> execBytecode ({frame with dataStack = newDataStack; fCode = {frame.fCode with co_code = CODE l}}))
-
-  | UNARY_NOT::l ->
-    let newDataStack = unary_not frame.dataStack in
-    let errCheck = check_err newDataStack in (
-    match errCheck with
-    | Some err -> err
-    | None -> execBytecode ({frame with dataStack = newDataStack; fCode = {frame.fCode with co_code = CODE l}}))
-
-  | BINARY_MULTIPLY::l -> 
-    let newDataStack = binary_multiply (frame.dataStack) in
-    let errCheck = check_err newDataStack in (
-    match errCheck with
-    | Some err -> err
-    | None -> execBytecode ({frame with dataStack = newDataStack; fCode = {frame.fCode with co_code = CODE l}}))
     
-  | BINARY_FLOOR_DIVIDE::l -> 
-    let newDataStack = binary_floor_divide (frame.dataStack) in
-    let errCheck = check_err newDataStack in (
-    match errCheck with
-    | Some err -> err
-    | None -> execBytecode ({frame with dataStack = newDataStack; fCode = {frame.fCode with co_code = CODE l}}))    
+(*
+   - Runs the code in the frame and update the VM once it's done.
+   Req: frame is the top element in the callstack in virM.
+*)
+let rec runFrame virM frame =
+  (* Execute the top frame *) 
+  let resultFrame = execBytecode frame in
+  let result = List.hd resultFrame.dataStack in
 
-  | BINARY_MODULO::l -> 
-    let newDataStack = binary_modulo (frame.dataStack) in
-    let errCheck = check_err newDataStack in (
-    match errCheck with
-    | Some err -> err
-    | None -> execBytecode ({frame with dataStack = newDataStack; fCode = {frame.fCode with co_code = CODE l}}))
+  (* Check if we spawn a new frame*)
+  match result with
+  | FRAMEOBJECT newFrame ->
+    let resultStack = {resultFrame with dataStack = List.tail resultFrame.dataStack} in
+    let newVM = {virM with callStack = resultFrame::(virM.callStack)} in
+    runFrame newVM newFrame
+  
+  | _ -> 
+    (* new global names*)
+    let new_globals = resultFrame.f_globals in
+    (* Pop the top frame *)
+    let popVM = {virM with callStack = List.tail (virM.callStack)} in
     
-  | BINARY_ADD::l -> 
-    let newDataStack = binary_add (frame.dataStack) in
-    let errCheck = check_err newDataStack in (
-    match errCheck with
-    | Some err -> err
-    | None -> execBytecode ({frame with dataStack = newDataStack; fCode = {frame.fCode with co_code = CODE l}}))    
-
-  | BINARY_SUBTRACT::l -> 
-    let newDataStack = binary_subtract (frame.dataStack) in
-    let errCheck = check_err newDataStack in (
-    match errCheck with
-    | Some err -> err
-    | None -> execBytecode ({frame with dataStack = newDataStack; fCode = {frame.fCode with co_code = CODE l}})) 
-    
-  | LOAD_CONST(i)::l ->
-    let newDataStack = load_const i (frame.fCode.co_consts) (frame.dataStack) in
-    let errCheck = check_err newDataStack in (
-    match errCheck with
-    | Some err -> err
-    | None -> execBytecode ({frame with dataStack = newDataStack; fCode = {frame.fCode with co_code = CODE l}}))
-    
-  | LOAD_FAST(i)::l ->
-    let newDataStack = load_fast i (frame.fCode.co_varnames) (frame.dataStack) in
-    let errCheck = check_err newDataStack in (
-    match errCheck with
-    | Some err -> err
-    | None ->  execBytecode ({frame with dataStack = newDataStack; fCode = {frame.fCode with co_code = CODE l}}))   
-    
-  | STORE_FAST(i)::l ->
-    let (newVarnames, newDataStack) = store_fast i (frame.fCode.co_varnames) (frame.dataStack) in
-    let newFCode = {frame.fCode with co_code = CODE l; co_varnames = newVarnames} in
-    let errCheck = check_err newDataStack in (
-    match errCheck with
-    | Some err -> err
-    | None -> execBytecode ({frame with dataStack = newDataStack; fCode = newFCode}))
-    
-    | [] -> All.failwith "Error: reached empty bytecode array "
-
+    (* Check if the top frame is the global frame *)
+    if List.length popVM.callStack = 0
+    then (popVM, result) 
+    else
+      (* Push result to the top of the caller frame (top frame in the call stack) *)
+      let callerFrame = List.hd popVM.callStack in
+      let newCallStack = List.tail popVM.callStack in
+      let newCallerFrame = {
+        callerFrame with 
+          dataStack =  result::callerFrame.dataStack;
+          pc = callerFrame.pc + 1;
+          f_globals = new_globals
+      } in
+      let newVM: vm = {popVM with callStack = newCallerFrame::newCallStack} in
+      runFrame newVM newCallerFrame
