VM.fst
@@ -1,42 +1,5 @@
-module VM 
-
-(* imported modules *)
-open Exec
-(* ---------------- *)
-
-(* Create a new frame and push it in the frame stack *)
-let makeFrame virM code =
-  let frame: frameObj = {dataStack = []; blockStack = []; fCode = code} in
-  let newVM: vm = {virM with callStack = frame::(virM.callStack)} in
-  (newVM, frame)
-
-
-(*
-   - Runs the code in the frame and update the VM once it's done.
-   Req: frame is the top element in the callstack in virM.
-*)
-let runFrame virM frame =
-  (* Execute *) 
-  let result = execBytecode frame in
-  result
-  
-  (*
-  
-  (* Check if result is ERR *)
-  
-  (* Pop the top frame*)
-  let popVM = {virM with callStack = List.tail (virM.callStack)} in
-  
-  (* Push result to the top of the caller frame (top frame in the call stack) *)
+module VM
  
-  let callerFrame = List.hd popVM.callStack in
-  let newCallStack = List.tail popVM.callStack in
-  let newCallerFrame = {callerFrame with dataStack =  result::callerFrame.dataStack} in
-  let newVM: vm = {popVM with callStack = newCallerFrame::newCallStack} in
-  (newVM, result)
-
-  *)
-
 (* Run code object *)
 let runCode code =
   (* Init the virtual machine *)
@@ -45,7 +8,10 @@ let runCode code =
     functionsEnv = []; 
     code = code
   } in
+  let empty_map = Map.const_on (Set.empty) NONE in
   (* Create global frame to run the byte code instructions in it *)
-  let  virM, globalFrame = makeFrame initVM code in
-  let  result = runFrame virM globalFrame in
+  let  virM, globalFrame = makeFrame initVM code [] empty_map empty_map in
+  let  finalVM, result = runFrame virM globalFrame in
   result
+  
+ 
