Exec.fsti
@@ -2,11 +2,12 @@ module Exec
 
 (* imported modules *)
 open Structs
+open Utils
 (* ---------------- *)
 
-val check_err: list pyObj -> All.ML (option pyObj) 
+val makeFrame: vm -> codeObj -> list pyObj -> (Map.t string pyObj) -> (Map.t string pyObj) -> (vm * frameObj)
 
-val return_value: list pyObj -> All.ML pyObj
+val call_function:  nat -> (Map.t string pyObj) -> list pyObj -> All.ML (list pyObj)
 
 val pop_top: list pyObj -> All.ML (list pyObj)
 
@@ -36,10 +37,34 @@ val binary_add: list pyObj -> All.ML (list pyObj)
 
 val binary_subtract: list pyObj -> All.ML (list pyObj)
 
+val binary_subscr: list pyObj -> All.ML (list pyObj)
+
+val store_name: nat -> list pyObj -> Map.t string pyObj -> list pyObj -> All.ML (Map.t string pyObj * list pyObj)
+
 val load_const: nat -> list pyObj -> list pyObj -> All.ML (list pyObj)
+
+val load_name: nat -> list pyObj -> Map.t string pyObj -> Map.t string pyObj -> list pyObj-> All.ML (list pyObj)
+
+val build_tuple: nat -> list pyObj -> All.ML (list pyObj)
+
+val build_list: nat -> list pyObj -> All.ML (list pyObj)
+
+val pop_jump_if_true: nat -> nat -> list pyObj -> All.ML (nat * list pyObj)
+
+val pop_jump_if_false: nat -> nat -> list pyObj -> All.ML (nat * list pyObj)
+
+val jump_if_true_or_pop: nat -> nat -> list pyObj -> All.ML (nat * list pyObj)
+
+val jump_if_false_or_pop: nat -> nat -> list pyObj -> All.ML (nat * list pyObj)
+
+val load_global: nat -> list pyObj -> Map.t string pyObj -> list pyObj-> All.ML (list pyObj)
 
 val load_fast: nat -> list pyObj -> list pyObj -> All.ML (list pyObj)
 
 val store_fast: nat -> list pyObj -> list pyObj -> All.ML (list pyObj * list pyObj)
 
-val execBytecode: frameObj -> All.ML pyObj
+val make_function: nat -> (Map.t string pyObj) ->list pyObj -> All.ML (list pyObj)
+
+val execBytecode: frameObj -> All.ML (frameObj)
+
+val runFrame: vm -> frameObj -> All.ML (vm * pyObj)
