Utils.fst
@@ -1,15 +1,47 @@
-module Utils 
+module Utils
 
 (* imported modules *)
 open Structs
 (* ---------------- *)
 
-
-let print_pyObj p =
+(*
+   Req: true
+*)
+let check_err dataStack = 
+  match (List.length dataStack) with
+  | 0 -> None
+  | _ ->
+    match (List.hd dataStack) with
+    | ERR(s) -> Some (ERR(s))
+    | _ -> None
+    
+let rec print_pyObj p: All.ML string =
   match p with
   | INT i -> Printf.sprintf "INT: %d" i
   | STRING s -> Printf.sprintf "STRING: %s" s
   | BOOL b ->  Printf.sprintf "BOOL: %b" b
+  | LIST l -> List.fold_right (fun a b -> a ^ " " ^ b) (List.map print_pyObj l) ""
+  | TUPLE l -> List.fold_right (fun a b -> a ^ " " ^ b) (List.map print_pyObj l) ""
   | NONE -> Printf.sprintf "NONE"
   | ERR s -> Printf.sprintf "ERR: %s" s
-  (*| _ -> Printf.sprintf ""*)
+  | _ -> Printf.sprintf "Not printable"
+
+let rec subString_pos' (cl: list String.char) (i: int): All.ML (option String.char) =
+  match cl with
+  | [] -> None
+  | x::cl' -> if i=0 then Some x else if i < 0 then None else (subString_pos' cl' (i-1))
+
+let subString_pos (s: string) (i: int): All.ML (option string) =
+  match (subString_pos' (String.list_of_string s) i) with
+  | None -> None
+  | Some c -> Some (String.string_of_char c)
+
+let subString_neg (s: string) (i: int): All.ML (option string) = subString_pos s ((String.length s) + i)
+
+let rec tabulate' (#a:Type) (f: nat -> a) (i: nat): list a =
+  match i with
+  | 0 -> []
+  | i -> (f (i-1))::(tabulate' f (i-1))
+
+let rec tabulate (#a:Type) (f: nat -> a) (i: nat): list a =
+  List.rev (tabulate' f i)
