VM.fsti
@@ -2,14 +2,8 @@ module VM
 
 (* imported modules *)
 open Structs
+open Exec
 (* ---------------- *)
-
-(* Creates a new frame and push it to the frame stack *)
-val makeFrame: vm -> codeObj ->  (vm * frameObj)
-
-(* Run Frame and then pop it from call stack when you done *)
-(* val runFrame: vm -> frameObj -> All.ML (vm * pyObj) *)
-val runFrame: vm -> frameObj -> All.ML pyObj
 
 (* Takes in code object and execute it *)
 val runCode: codeObj -> All.ML pyObj
